src/SoftBound/sb_db_trans.v
@@ -74,14 +74,18 @@ match i with
 | insn_fcmp _ _ _ _ _ => Some (typ_int Size.One)
 | insn_select _ _ typ _ _ => Some typ
 | insn_call _ true _ typ _ _ => Some typ_void
-| insn_call _ false _ typ _ _ => Some typ
+| insn_call _ false _ typ _ _ => 
+    match typ with
+    | typ_function t _ _ => Some t
+    | _ => None
+    end
 end.
 
 Definition rmap := list (id*(id*id)).
 
 Definition getFdefIDs fdef : ids :=
 match fdef with
-| fdef_intro (fheader_intro _ _ la) bs => 
+| fdef_intro (fheader_intro _ _ la _) bs => 
   let '(_, ids0) := List.split la in
   ids0 ++ getBlocksIDs bs 
 end.
@@ -146,7 +150,7 @@ end.
 
 Definition gen_metadata_fdef nts (ex_ids:ids) (rm:rmap) (f:fdef) 
   : option(ids*rmap) :=
-let '(fdef_intro (fheader_intro _ _ la) bs) := f in
+let '(fdef_intro (fheader_intro _ _ la _) bs) := f in
 let '(ex_ids', rm') := gen_metadata_args ex_ids rm la in
 gen_metadata_blocks nts ex_ids' rm' bs.
 
@@ -175,40 +179,40 @@ Parameter fake_id : id.
 Parameter get_mmetadata_fid : id.
 Parameter set_mmetadata_fid : id.
 
-Definition assert_mptr_fn : value :=
-  value_const
-    (const_gid 
-      (typ_function typ_void 
+Definition assert_mptr_typ : typ :=
+  typ_function typ_void 
         (Cons_list_typ p8 
         (Cons_list_typ p8 
         (Cons_list_typ p8
         (Cons_list_typ i32
-        (Cons_list_typ i32 Nil_list_typ))))))
-      assert_mptr_fid).
+        (Cons_list_typ i32 Nil_list_typ))))) false.
 
-Definition get_mmetadata_fn : value :=
-  value_const
-    (const_gid 
-      (typ_function typ_void 
+Definition assert_mptr_fn : value :=
+  value_const (const_gid assert_mptr_typ assert_mptr_fid).
+
+Definition get_mmetadata_typ : typ :=
+  typ_function typ_void 
         (Cons_list_typ p8 
         (Cons_list_typ pp8 
         (Cons_list_typ pp8
         (Cons_list_typ p8
         (Cons_list_typ i32
-        (Cons_list_typ p32 Nil_list_typ)))))))
-      get_mmetadata_fid).
+        (Cons_list_typ p32 Nil_list_typ)))))) false.
 
-Definition set_mmetadata_fn : value :=
-  value_const
-    (const_gid 
-      (typ_function typ_void 
+Definition get_mmetadata_fn : value :=
+  value_const (const_gid get_mmetadata_typ get_mmetadata_fid).
+
+Definition set_mmetadata_typ : typ :=
+  typ_function typ_void 
         (Cons_list_typ p8 
         (Cons_list_typ p8 
         (Cons_list_typ p8
         (Cons_list_typ p8
         (Cons_list_typ i32
-        (Cons_list_typ i32 Nil_list_typ)))))))
-      set_mmetadata_fid).
+        (Cons_list_typ i32 Nil_list_typ)))))) false.
+
+Definition set_mmetadata_fn : value :=
+  value_const (const_gid set_mmetadata_typ set_mmetadata_fid).
 
 Definition prop_metadata (ex_ids tmps:ids) (optaddrb optaddre: option id) rm c v1
   id0 :=
@@ -292,7 +296,8 @@ match c with
               match (optaddrb, optaddre) with
               | (Some addrb, Some addre) =>
                    (Some
-                     (insn_call fake_id true false typ_void get_mmetadata_fn 
+                     (insn_call fake_id true false 
+                       get_mmetadata_typ get_mmetadata_fn 
                        ((p8,(value_id ptmp))::
                         (pp8,(value_id addrb))::
                         (pp8,(value_id addre))::
@@ -307,7 +312,8 @@ match c with
                    let '(addrb,ex_ids) := mk_tmp ex_ids in
                    let '(addre,ex_ids) := mk_tmp ex_ids in
                    (Some
-                     (insn_call fake_id true false typ_void get_mmetadata_fn 
+                     (insn_call fake_id true false 
+                       get_mmetadata_typ get_mmetadata_fn 
                        ((p8,(value_id ptmp))::
                         (pp8,(value_id addrb))::
                         (pp8,(value_id addre))::
@@ -330,7 +336,7 @@ match c with
          insn_cast ptmp castop_bitcast (typ_pointer t2) v2 p8:: 
          insn_cast btmp castop_bitcast mt bv p8:: 
          insn_cast etmp castop_bitcast mt ev p8:: 
-         insn_call fake_id true false typ_void assert_mptr_fn 
+         insn_call fake_id true false assert_mptr_typ assert_mptr_fn 
            ((p8,(value_id btmp))::
             (p8,(value_id etmp))::
             (p8,(value_id ptmp))::
@@ -353,7 +359,7 @@ match c with
           match get_reg_metadata rm v1 with
           | Some (mt1, bv0, ev0) =>
               Some
-                (insn_call fake_id true false typ_void set_mmetadata_fn 
+                (insn_call fake_id true false set_mmetadata_typ set_mmetadata_fn 
                   ((p8,(value_id ptmp))::
                    (p8,bv0)::
                    (p8,ev0)::
@@ -372,7 +378,7 @@ match c with
          insn_cast ptmp castop_bitcast (typ_pointer t0) v2 p8:: 
          insn_cast btmp castop_bitcast mt2 bv p8:: 
          insn_cast etmp castop_bitcast mt2 ev p8:: 
-         insn_call fake_id true false typ_void assert_mptr_fn 
+         insn_call fake_id true false assert_mptr_typ assert_mptr_fn 
            ((p8,(value_id btmp))::
             (p8,(value_id etmp))::
             (p8,(value_id ptmp))::
@@ -590,7 +596,7 @@ match (optaddrb, optaddre) with
 end.
 
 Definition trans_fdef nts (f:fdef) : option fdef :=
-let '(fdef_intro (fheader_intro t fid la) bs) := f in
+let '(fdef_intro (fheader_intro t fid la va) bs) := f in
 if SimpleSE.isCallLib fid then Some f
 else
   let ex_ids := getFdefIDs f in
@@ -601,7 +607,7 @@ else
           match (trans_blocks ex_ids nil None None rm bs) with
           | Some (ex_ids, tmps, optaddrb, optaddre, b'::bs') => 
               Some (fdef_intro 
-                     (fheader_intro t (rename_fid fid) (la++la')) 
+                     (fheader_intro t (rename_fid fid) (la++la') va) 
                      ((insert_more_allocas optaddrb optaddre b')::bs'))
           | _ => None
           end
@@ -761,7 +767,7 @@ Mem.mem_inj mi Mem1 Mem2 /\
   getOperandValue TD Mem2 v lc2 gl = Some pgv' ->
   exists bgv', exists egv', exists Mem2',
   SimpleSE.dbCmds TD gl lc2 als Mem2
-    (insn_call fake_id true false typ_void get_mmetadata_fn 
+    (insn_call fake_id true false get_mmetadata_typ get_mmetadata_fn 
        ((p8,v)::
         (p8,(value_id addrb))::
         (p8,(value_id addre))::nil)::
@@ -841,7 +847,7 @@ Axiom get_mmetadata_fn__alloc : forall
   (egv' : GenericValue)
   (Mem21 : mem)
   (J37 : dbCmds TD gl lc2 als Mem2
-          (insn_call fake_id true false typ_void get_mmetadata_fn
+          (insn_call fake_id true false get_mmetadata_typ get_mmetadata_fn
              ((p8, v)
               :: (p8, value_id addrb0) :: (p8, value_id addre0) :: nil)
            :: insn_load bid0 p8 (value_id addrb0) Align.Zero
@@ -850,7 +856,7 @@ Axiom get_mmetadata_fn__alloc : forall
              eid0 egv') als Mem21 trace_nil),
    exists Mem21' : mem,
      dbCmds TD gl lc2 als Mem2'
-       (insn_call fake_id true false typ_void get_mmetadata_fn
+       (insn_call fake_id true false get_mmetadata_typ get_mmetadata_fn
           ((p8, v) :: (p8, value_id addrb0) :: (p8, value_id addre0) :: nil)
         :: insn_load bid0 p8 (value_id addrb0) Align.Zero
            :: insn_load eid0 p8 (value_id addre0) Align.Zero :: nil)
@@ -901,7 +907,7 @@ Axiom assert_mptr_fn__ok : forall
      (updateAddAL GenericValue
         (updateAddAL GenericValue (updateAddAL GenericValue lc2 ptmp gvp2)
            btmp bgv2) etmp egv2) als Mem2
-     (insn_call fake_id true false typ_void assert_mptr_fn
+     (insn_call fake_id true false assert_mptr_typ assert_mptr_fn
         ((p8, value_id btmp)
          :: (p8, value_id etmp)
             :: (p8, value_id ptmp)
@@ -932,7 +938,7 @@ Axiom get_mmetadata_fn__weaken : forall
   (egv' : GenericValue)
   (Mem2' : mem)
   (JJ1 : dbCmds TD gl lc2 als Mem2
-          (insn_call fake_id true false typ_void get_mmetadata_fn
+          (insn_call fake_id true false get_mmetadata_typ get_mmetadata_fn
              ((p8, vp) :: (p8, value_id addrb) :: (p8, value_id addre) :: nil)
            :: insn_load bid0 p8 (value_id addrb) Align.Zero
               :: insn_load eid0 p8 (value_id addre) Align.Zero :: nil)
@@ -945,7 +951,7 @@ Axiom get_mmetadata_fn__weaken : forall
         (updateAddAL GenericValue
            (updateAddAL GenericValue (updateAddAL GenericValue lc2 ptmp gvp2)
               btmp bgv2) etmp egv2) id0 gv2) als Mem2
-     (insn_call fake_id true false typ_void get_mmetadata_fn
+     (insn_call fake_id true false get_mmetadata_typ get_mmetadata_fn
         ((p8, value_id ptmp)
          :: (pp8, value_id addrb)
             :: (pp8, value_id addre)
@@ -964,7 +970,7 @@ Axiom get_mmetadata_fn__prop : forall m Mem2 b2 ofs2 v1 Mem2' lc2 gl als addrb
     addre bid0 eid0 bgv' egv' Mem3 TD v,
   Mem.store m Mem2 b2 ofs2 v = ret Mem2' ->
   dbCmds TD gl lc2 als Mem2
-         (insn_call fake_id true false typ_void get_mmetadata_fn
+         (insn_call fake_id true false get_mmetadata_typ get_mmetadata_fn
             ((p8, v1) :: (p8, value_id addrb) :: (p8, value_id addre) :: nil)
           :: insn_load bid0 p8 (value_id addrb) Align.Zero
              :: insn_load eid0 p8 (value_id addre) Align.Zero :: nil)
@@ -972,7 +978,7 @@ Axiom get_mmetadata_fn__prop : forall m Mem2 b2 ofs2 v1 Mem2' lc2 gl als addrb
             eid0 egv') als Mem3 trace_nil ->
    exists Mem2'0 : mem,
      dbCmds TD gl lc2 als Mem2'
-       (insn_call fake_id true false typ_void get_mmetadata_fn
+       (insn_call fake_id true false get_mmetadata_typ get_mmetadata_fn
           ((p8, v1) :: (p8, value_id addrb) :: (p8, value_id addre) :: nil)
         :: insn_load bid0 p8 (value_id addrb) Align.Zero
            :: insn_load eid0 p8 (value_id addre) Align.Zero :: nil)
@@ -984,7 +990,7 @@ Axiom set_mmetadata_fn__prop : forall TD gl lc2 als Mem2 ptmp pgv' bv0 ev0,
   lookupAL _ lc2 ptmp = Some pgv' ->
   exists Mem2',
     SimpleSE.dbCmd TD gl lc2 als Mem2
-      (insn_call fake_id true false typ_void set_mmetadata_fn
+      (insn_call fake_id true false set_mmetadata_typ set_mmetadata_fn
         ((p8, value_id ptmp) :: (p8, bv0) :: (p8, ev0) :: (p8, vnullp8) :: 
          (i32, vint1) :: (i32, vint1) :: nil)) 
       lc2 als Mem2' trace_nil /\
@@ -1002,7 +1008,7 @@ Axiom set_mmetadata_fn__getOperandValue : forall
   (TD : TargetData)
   (Mem2' : mem)
   (J : dbCmd TD gl lc2 als Mem2
-        (insn_call fake_id true false typ_void set_mmetadata_fn
+        (insn_call fake_id true false set_mmetadata_typ set_mmetadata_fn
            ((p8, value_id ptmp)
             :: (p8, bv0)
                :: (p8, ev0)
@@ -1032,7 +1038,7 @@ Axiom get_set_mmetadata_fn : forall
   (Hgete : getOperandValue TD Mem2 ev0 lc2 gl = ret egv')
   (Mem2' : mem)
   (J : dbCmd TD gl lc2 als Mem2
-        (insn_call fake_id true false typ_void set_mmetadata_fn
+        (insn_call fake_id true false set_mmetadata_typ set_mmetadata_fn
            ((p8, value_id ptmp)
             :: (p8, bv0)
                :: (p8, ev0)
@@ -1055,7 +1061,7 @@ Axiom get_set_mmetadata_fn : forall
   (Hinjp : gv_inject mi (ptr2GV TD (Vptr b ofs0)) pgv'),
   exists Mem2'0 : mem,
      dbCmds TD gl0 lc0 als0 Mem2'
-       (insn_call fake_id true false typ_void get_mmetadata_fn
+       (insn_call fake_id true false get_mmetadata_typ get_mmetadata_fn
           ((p8, v0) :: (p8, value_id addrb) :: (p8, value_id addre) :: nil)
         :: insn_load bid0 p8 (value_id addrb) Align.Zero
            :: insn_load eid0 p8 (value_id addre) Align.Zero :: nil)
@@ -1065,7 +1071,7 @@ Axiom get_set_mmetadata_fn : forall
 
 Axiom set_mmetadata_fn__prop' : forall TD gl lc1 Mem1 args lc2 als Mem2,
   dbCmd TD gl lc1 als Mem1 
-    (insn_call fake_id true false typ_void set_mmetadata_fn args)
+    (insn_call fake_id true false set_mmetadata_typ set_mmetadata_fn args)
     lc2 als Mem2 trace_nil ->
   Mem.nextblock Mem1 <= Mem.nextblock Mem2 /\
   (forall b2, Mem.valid_block Mem1 b2 -> Mem.valid_block Mem2 b2) /\
@@ -1075,7 +1081,7 @@ Axiom get_mmetadata_fn__prop' : forall Mem2 b lo hi v1 Mem2' lc2 gl als addrb
     addre bid0 eid0 bgv' egv' Mem3 TD,
   Mem.free Mem2 b lo hi = ret Mem2' ->
   dbCmds TD gl lc2 als Mem2
-         (insn_call fake_id true false typ_void get_mmetadata_fn
+         (insn_call fake_id true false get_mmetadata_typ get_mmetadata_fn
             ((p8, v1) :: (p8, value_id addrb) :: (p8, value_id addre) :: nil)
           :: insn_load bid0 p8 (value_id addrb) Align.Zero
              :: insn_load eid0 p8 (value_id addre) Align.Zero :: nil)
@@ -1083,7 +1089,7 @@ Axiom get_mmetadata_fn__prop' : forall Mem2 b lo hi v1 Mem2' lc2 gl als addrb
             eid0 egv') als Mem3 trace_nil ->
    exists Mem2'0 : mem,
      dbCmds TD gl lc2 als Mem2'
-       (insn_call fake_id true false typ_void get_mmetadata_fn
+       (insn_call fake_id true false get_mmetadata_typ get_mmetadata_fn
           ((p8, v1) :: (p8, value_id addrb) :: (p8, value_id addre) :: nil)
         :: insn_load bid0 p8 (value_id addrb) Align.Zero
            :: insn_load eid0 p8 (value_id addre) Align.Zero :: nil)
